mppa_k1c/SelectOpproof.v
@@ -582,22 +582,22 @@ Proof.
     inv H2. inv H5.
     replace v8 with v4 in * by congruence.
     rename v4 into vselect.
-    destruct vselect; simpl; trivial.
-    rewrite (Val.and_commut _ v5).
-    destruct v5; simpl; trivial.
-    rewrite (Val.and_commut _ v9).
-    rewrite Val.or_commut.
-    destruct v9; simpl; trivial.
-    rewrite int_eq_commut.
-    destruct (Int.eq i1 Int.zero); simpl.
-    + rewrite Int.and_zero.
-      rewrite Int.or_commut.
-      rewrite Int.or_zero.
+    destruct vselect; simpl; trivial;
+    destruct v5; simpl; trivial; destruct v9; simpl; trivial;
+    destruct (Int.eq i1 Int.zero); simpl; trivial.
+    + rewrite Int.neg_zero.
+      rewrite Int.and_commut.
       rewrite Int.and_mone.
-      reflexivity.
-    + rewrite Int.and_mone.
-      rewrite Int.neg_zero.
+      rewrite Int.and_commut.
       rewrite Int.and_zero.
+      rewrite Int.or_zero.
+      reflexivity.
+    + rewrite Int.neg_zero.
+      rewrite Int.and_commut.
+      rewrite Int.and_zero.
+      rewrite Int.and_commut.
+      rewrite Int.and_mone.
+      rewrite Int.or_commut.
       rewrite Int.or_zero.
       reflexivity.
   - (* select unsigned *)
@@ -620,22 +620,23 @@ Proof.
     inv H2. inv H5.
     replace v8 with v4 in * by congruence.
     rename v4 into vselect.
-    destruct vselect; simpl; trivial.
-    rewrite (Val.and_commut _ v5).
-    destruct v5; simpl; trivial.
-    rewrite (Val.and_commut _ v9).
-    rewrite Val.or_commut.
-    destruct v9; simpl; trivial.
-    rewrite int_eq_commut.
-    destruct (Int.eq i1 Int.zero); simpl.
-    + rewrite Int.and_zero.
-      rewrite Int.or_commut.
-      rewrite Int.or_zero.
+    destruct vselect; simpl; trivial;
+    destruct v5; simpl; trivial;
+    destruct v9; simpl; trivial;
+    destruct (Int.eq i1 Int.zero); simpl; trivial.
+    + rewrite Int.neg_zero.
+      rewrite Int.and_commut.
       rewrite Int.and_mone.
-      reflexivity.
-    + rewrite Int.and_mone.
-      rewrite Int.neg_zero.
+      rewrite Int.and_commut.
       rewrite Int.and_zero.
+      rewrite Int.or_zero.
+      reflexivity.
+    + rewrite Int.neg_zero.
+      rewrite Int.and_commut.
+      rewrite Int.and_zero.
+      rewrite Int.and_commut.
+      rewrite Int.and_mone.
+      rewrite Int.or_commut.
       rewrite Int.or_zero.
       reflexivity.
   - apply DEFAULT.
